src/study/Nemonuri.Study.CSharpSyntaxRewriter2.Modifier/Nemonuri.StratifiedNode.TypeTheory1.fst
@@ -28,6 +28,15 @@ open Nemonuri.StratifiedNode
 open Nemonuri.StratifiedNode.NodeTheory
 open Nemonuri.StratifiedNode.ListTheory
 
+private let lemma_for_all
+  (#t:eqtype) (#mlv:nat) (snl:stratified_node_list t mlv{SCons? snl})
+  (#lv:pos) (sn:stratified_node t lv)
+  (predicate:stratified_node_predicate t)
+  : Lemma (requires (for_all snl predicate) && (contains snl sn))
+          (ensures predicate sn)
+          (decreases snl)
+  = lemma_list_satisfies_for_all_predicate_means_element_satisfies_predicate snl sn predicate; ()
+
 type argument_sum_kind =
   | Argument_s0
   | Argument_s1
@@ -62,10 +71,6 @@ let get_argument_sum_kind (#lv:pos) (sn:node lv{ is_kind_argument sn })
   : Tot argument_sum_kind
   = let Argument v0 = (get_kind sn) in v0
 
-let is_kind_argument_s0 (#lv:pos) (sn:node lv)
-  : Tot bool
-  = (is_kind_argument sn) && (Argument_s0? (get_argument_sum_kind sn)) //TODO: block block*
-
 let is_kind_argument_s1 (#lv:pos) (sn:node lv)
   : Tot bool
   = (is_kind_argument sn) && 
@@ -73,11 +78,32 @@ let is_kind_argument_s1 (#lv:pos) (sn:node lv)
     (get_children_length sn = 1) &&
     (is_kind_blockless_expression (get_child_at sn 0))
 
-(*
 let is_kind_statement (#lv:pos) (sn:node lv)
   : Tot bool
-  = 
-*)
+  = (Statement? (get_kind sn)) &&
+    (for_all sn.children is_kind_argument)
+
+let is_kind_block (#lv:pos) (sn:node lv)
+  : Tot bool
+  = (Block? (get_kind sn)) &&
+    (for_all sn.children is_kind_statement)
+
+let is_kind_compilation_unit (#lv:pos) (sn:node lv)
+  : Tot bool
+  = (Compilation_unit? (get_kind sn)) &&
+    (for_all sn.children is_kind_block)
+
+let is_kind_argument_s0 (#lv:pos) (sn:node lv)
+  : Tot bool
+  = (is_kind_argument sn) && 
+    (Argument_s0? (get_argument_sum_kind sn)) &&
+    (get_children_length sn >= 1) &&
+    (for_all sn.children is_kind_block)
+
+private let lemma_test
+  (#lv:pos) (sn:node lv{ is_kind_compilation_unit sn && get_children_length sn >= 3 })
+  : Lemma (is_kind_block (get_child_at sn 2))
+  = ()
 
 (*
 let is_kind_argument_s1 (#lv:pos) (sn:node lv)
